our_cook/op_correspond.v
@@ -1,9 +1,190 @@
 Require Import Coq.Lists.List.
 Import ListNotations.
 Require Import Coq.Relations.Relation_Operators. 
+From Coq Require Import Lia.
+Require Import PeanoNat.
 From Encoding Require Export cbpv.
 From Encoding Require Export pi.
 From Encoding Require Export encoding.
+
+Lemma links: forall s n m,
+  (Res (Res (Par 
+    (encode s 1 0 [])
+    (Par
+      (Link 1 (n + 2))
+      (Link 0 (m + 2))
+    )
+  ))) ~~
+  (encode s n m []).
+Proof.
+Admitted.
+
+Lemma stuff: forall s u r,
+  (Res ^^ 6)
+    (Par
+       (Par (encode s 1 0 [])
+          (Rep (In 0 (In 0 (In 1 (encode s 1 0 [])))) [[shift]] [[shift]] [[shift]]))
+       (Par (Link 1 (u + 6)) (Link 0 (r + 6)))) ~~ 
+  ((Res ^^ 6) (Par
+    (encode s 1 0 [])
+    (Par (Link 1 (u + 6)) (Link 0 (r + 6)))
+  )).
+Proof.
+Admitted.
+
+Lemma res_encoding: forall s u r,
+  (Res (encode s (u + 1) (r + 1) [])) ~~ (encode s u r []).
+Proof.
+  cofix CH.
+  intros s.
+  induction s.
+  - induction v.
+    * intros u r.
+      simpl.
+      apply wb.
+      intros a p' Htrans.
+      + { induction a.
+          - inversion Htrans.
+            contradiction.
+            inversion H0.
+          - inversion Htrans.
+            inversion H1.
+          - destruct (Nat.eq_dec n0 u) as [Heq | Hneq].
+            * subst n0.
+              exists 
+                (Rep (In 0 (In 0 (In 1 (In (n + 4)
+                  (In 0 (In 1 (Par (Link 1 4) (Link 0 3))))))))).
+              split.
+              + eapply WT_VIS.
+                discriminate.
+                apply rt_refl.
+                apply OUT.
+                apply rt_refl.
+              + inversion Htrans. 
+            
+        }
+Admitted.
+
+Lemma res_n_encoding:
+forall n s u r,
+  ((Res ^^ n) (encode s (u + n) (r + n) [])) ~~ (encode s u r []).
+Proof.
+  intros n.
+  induction n.
+  - intros s u r.
+    simpl.
+    replace (u + 0) with u by lia.
+    replace (r + 0) with r by lia.
+    apply wb_ref.
+  - intros s u r.
+    eapply wb_trans.
+    * simpl.
+      replace (u + S n) with ((u + 1) + n) by lia.
+      replace (r + S n) with ((r + 1) + n) by lia.
+      apply wb_res.
+      apply IHn.
+    * apply res_encoding.
+Qed.
+
+Lemma force_thunk_sound: 
+forall s u r,
+  exists P,
+    encode (Force (Thunk s)) u r [] =()> P /\ P ~~ encode s u r [].
+Proof.
+  intros s u r.
+  exists ((Res ^^ 6)(Par
+    (Par 
+      (encode s 1 0 [])
+      (Rep
+        (In 0 (In 0 (In 1 (encode s 1 0 [])))) 
+        [[shift]] [[shift]] [[shift]]
+      )
+    )
+    (Par 
+      (Link 1 (u + 6)) 
+      (Link 0 (r + 6))
+    )
+  )).
+  split.
+  * eapply rt_trans.
+    apply rt_step.
+    simpl.
+    repeat (apply RES_TAU).
+    { apply COM with
+        (a := a_out 1)
+        (R := Rep (In 0 (In 0 (In 1 (encode s 1 0 [])))))
+        (S := Out 0 (Out 0 (Out 1 (Par (Link 1 (u + 6)) (Link 0 (r + 6)))))).
+      - exact 0.
+      - discriminate.
+      - apply OUT.
+      - apply IN.
+    }
+    + { eapply rt_trans.
+        - apply rt_step.
+          repeat (apply RES_TAU).
+          apply COM with
+            (a := a_in 0)
+            (R := Par
+              (In 0 (In 1 (encode s 1 0 [])))
+              (Rep (In 0 (In 0 (In 1 (encode s 1 0 [])))) [[shift]])
+            )
+            (S := Out 0 (Out 1 (Par (Link 1 (u + 6)) (Link 0 (r + 6))))).
+          * exact 0.
+          * discriminate.
+          * apply REP.
+            eapply PAR_L.
+            + discriminate.
+            + apply IN.
+          * simpl.
+            apply OUT.
+        - eapply rt_trans.
+          * apply rt_step.
+            repeat (apply RES_TAU).
+            apply COM with
+              (a := a_in 0)
+              (R := Par
+                (In 1 (encode s 1 0 []))
+                (Rep (In 0 (In 0 (In 1 (encode s 1 0 [])))) [[shift]] [[shift]])
+              )
+              (S := Out 1 (Par (Link 1 (u + 6)) (Link 0 (r + 6)))).
+            + exact 0.
+            + discriminate.
+            + { apply PAR_L.
+                - discriminate.
+                - apply IN.
+              }
+            + simpl.
+              apply OUT.
+         * eapply rt_trans.
+           + apply rt_step.
+             repeat (apply RES_TAU).
+             { apply COM with
+                 (a := a_in 1)
+                 (R := Par
+                   (encode s 1 0 [])
+                   (Rep (In 0 (In 0 (In 1 (encode s 1 0 [])))) [[shift]] [[shift]] [[shift]])
+                 )
+                 (S := Par (Link 1 (u + 6)) (Link 0 (r + 6))).
+               - exact 0.
+               - discriminate.
+               - apply PAR_L.
+                 * discriminate.
+                 * apply IN.
+               - apply OUT.
+             }
+           + apply rt_refl.
+     }
+  * eapply wb_trans.
+    + apply stuff.
+    + { eapply wb_trans.
+        - do 4 (apply wb_res).
+          replace (u + 6) with ((u + 4) + 2) by lia.
+          replace (r + 6) with ((r + 4) + 2) by lia.
+          apply links.
+        - fold ((Res ^^ 4) (encode s (u + 4) (r + 4) [])).
+          apply res_n_encoding.
+      }
+Qed.
 
 Theorem sound: forall s t, 
   s --> t -> 
@@ -15,25 +196,9 @@ Proof.
   induction Hred.
   - admit.
   - admit.
-  - intros u r.
-    exists (encode s u r []).
-    split.
-    * eapply rt_trans.
-      + apply rt_step.
-        simpl.
-        apply RES_TAU.
-        apply RES_TAU.
-        { apply COM with
-            (a := a_out 0)
-            (R := Rep (In 0 (In 0 (In 1 (encode s 1 0 [])))))
-            (S := Out 0 (Out 0 (Out 1 (Par (Link 1 (u + 6)) (Link 0 (r + 6)))))).
-          - exact 0.
-          - discriminate.
-          - admit.
-          - simpl.
-        }  
-        
-    * apply wb_ref.
+  - apply force_thunk_sound.
+  - admit.
+  - admit.
 Admitted.
 
 Theorem complete: forall s P u r, 
